# 9.2 Lenses Categorically
van Laarhoven representation of a lens:
```
  type Lens s t a b = forall f . Functor f => (a -> f b) -> s -> f t
```
Let's rewrite this in a more convenient format
```
  s -> forall f . (a -> f b) -> f t
```
Since this is true for *all* functors, we can only use `fmap`. We need an `a` and a function `b -> t`. This is `IStore`!
```
  s -> IStore a b t
```

## Yoneda embedding
```
  [C, Set](C(a, _), C(b, _)) ~ C(b, a)
  forall c . (a -> c) -> (b -> c) ~ b -> a
```
This only talks about objects in `C`, but we want to talk about functors on `C`. We'll restrict our focus to endofunctors.

```
  [[C, C], Set]([C, C](g, _), [C, C](h, _)) ~ [C, C](h, g)
  forall f . Functor => (forall c . g c -> f c) -> (forall c' . h c' -> f c') ~ forall c . h c -> g c
```

## Adjunctions
```
  [C, D]
  C(L d, c) ~ D(d, R c)
```
In a functor category, we have
```
  [C, C](L g, f) ~ [C, C](g, R f)
  forall c . (L g) c -> f c ~ forall c' . g c' -> R f c'
```

Now rewriting the functor category Yoneda embedding with `L g` and `L' h` instead
```
  forall f . Functor => (forall c . (L g) c -> f c) -> (forall c' . (L' h) c' -> f c') ~ forall c . (L' h) c -> (L g) c
```
and then using the adjunctions `L -| R` and `L' -| R'`, we get
```
  forall f . Functor => (forall c . g c -> (R f) c) -> (forall c' . h c' -> (R' f) c') ~ forall c . h c -> (R' (L g)) c
```

Now we make `g` and `h` hom-functors, i.e. `g = C(b, _)` and `h = C(t, _)`
```
  forall f . Functor => (forall c . (b -> c) -> (R f) c) -> (forall c' . (t -> c') -> (R' f) c') ~ forall c . (t -> c) -> (R' (L g)) c
```

Aha! Now we are in a position to apply the Yoneda lemma again!
```
  forall f . Functor => (R f) b -> (R' f) t ~ (R' (L g)) t
```

We want: `(R f) b = a -> f b` (`a -> f b` is a profunctor in `(a, b)`, *up star*) and `(R' f) t = (s -> f t)`

So the left side of the isomorphism is the van Laarhoven representation of a lens. Next, we show that the right side is (isomorphic to) the original notion of a lens.
```
  (R' (L g)) t = s -> (L g) t
```
Recall that the adjunction `L -| R` means
```
  forall c . (L g) c -> f c ~ forall c . g c -> (R f) c
```
and `g c -> (R f) c = g c -> a -> f c ~ (a, g c) -> f c`. So by making `L g = (a, g _)`, we get
```
  (R' (L g)) t = s -> (a, g t) = (a, b -> t)
```
i.e. getter and setter.
